wip

crypto/bignum/Hacl.Bignum.Fdifference.fst
@@ -10,23 +10,40 @@ open Hacl.Bignum.Limb
 
 module U32 = FStar.UInt32
 
-let gte_felem h (b:felem) h' (b':felem) (l:nat{l <= len}) : GTot Type0 =
-  live h b /\ live h' b'
-  /\ (forall (i:nat). {:pattern (get h b i) \/ (get h' b' i)} i < l ==> v (get h b i) >= v (get h' b' i))
+type seqelem = s:Seq.seq limb{Seq.length s = len}
 
 
-let is_subtraction h (b:felem) h' (b':felem) (l:nat{l <= len}) : GTot Type0 =
-  live h b /\ live h' b /\ live h' b'
-  /\ (forall (i:nat). {:pattern (get h b i)} (i >= l /\ i < len) ==> v (get h b i) = v (get h' b' i) - v (get h' b i))
+let gte_limbs (a:seqelem) (b:seqelem) (l:nat{l <= len}) : GTot Type0 =
+  (forall (i:nat). {:pattern (Seq.index a i) \/ (Seq.index b i)} i < l ==> v (Seq.index b i) >= v (Seq.index a i))
+
+
+val fdifference_spec:
+  a:seqelem -> b:seqelem ->
+  ctr:nat{ctr <= len /\ gte_limbs a b ctr} ->
+  Tot seqelem (decreases ctr)
+let rec fdifference_spec a b ctr =
+  if ctr = 0 then a
+  else (
+    let i = ctr - 1 in
+    let ai = Seq.index a i in
+    let bi = Seq.index b i in
+    let a' = Seq.upd a i (bi -^ ai) in
+    fdifference_spec a' b i
+  )
+
+
+let gte_limbs_c h (a:felem) h' (b:felem) (l:nat{l <= len}) : GTot Type0 =
+  live h a /\ live h' b /\ gte_limbs (as_seq h a) (as_seq h' b) l
 
 
 val fdifference_:
   a:felem ->
-  b:felem ->
-  i:ctr ->
+  b:felem{disjoint a b} ->
+  i:ctr{U32.v i <= len} ->
   Stack unit
-    (requires (fun h -> true))
-    (ensures (fun _ _ _ -> true))
+    (requires (fun h -> gte_limbs_c h a h b (U32.v i)))
+    (ensures (fun h0 _ h1 -> gte_limbs_c h0 a h0 b (U32.v i) /\ live h1 a
+      /\ as_seq h1 a == fdifference_spec (as_seq h0 a) (as_seq h0 b) (U32.v i)))
 let rec fdifference_ a b i =
   if U32 (i =^ 0ul) then ()
   else (
@@ -37,11 +54,11 @@ let rec fdifference_ a b i =
   )
 
 
-val fdifference:
-  a:felem ->
-  b:felem ->
-  Stack unit
-    (requires (fun h -> gte_felem h b h a len))
-    (ensures  (fun h0 _ h1 -> is_subtraction h1 a h0 b 0))
-let fdifference a b =
-  fdifference_ a b clen
+(* val fdifference: *)
+(*   a:felem -> *)
+(*   b:felem -> *)
+(*   Stack unit *)
+(*     (requires (fun h -> gte_limbs_c h b h a len)) *)
+(*     (ensures  (fun h0 _ h1 -> is_subtraction h1 a h0 b 0)) *)
+(* let fdifference a b = *)
+(*   fdifference_ a b clen *)
