crypto/bignum/Hacl.Bignum.Fsum.fst
@@ -6,22 +6,49 @@ open FStar.Buffer
 open Hacl.Bignum.Parameters
 open Hacl.Bignum.Bigint
 open Hacl.Bignum.Limb
+open Hacl.Bignum.Predicates
 
 
 module U32 = FStar.UInt32
 
+
+type seqelem = s:Seq.seq limb{Seq.length s = len}
+
+
+let red (s:seqelem) (l:nat{l <= len}) = (forall (i:nat). (i < l) ==> v (Seq.index s i) < pow2 (n - 1))
+
+
+val fsum_spec: s:seqelem -> s':seqelem -> ctr:nat{ctr <= len /\ red s ctr /\ red s' ctr} -> Tot seqelem
+  (decreases ctr)
+let rec fsum_spec a b ctr =
+  if ctr = 0 then a
+  else (
+    let i = ctr - 1 in
+    let ai = Seq.index a i in
+    let bi = Seq.index b i in
+    Math.Lemmas.pow2_double_sum (n-1);
+    let a' = Seq.upd a i (ai +^ bi) in
+    fsum_spec a' b i
+  )
+
+
+let red_c h (f:felem) ctr = live h f /\ red (as_seq h f) ctr
+
+
 val fsum_:
-  felem ->
-  felem ->
-  ctr ->
+  a:felem ->
+  b:felem{disjoint a b} ->
+  i:ctr{U32.v i <= len} ->
   Stack unit
-    (requires (fun _ -> True))
-    (ensures (fun _ _ _ -> true))
+    (requires (fun h -> red_c h a (U32.v i) /\ red_c h b (U32.v i)))
+    (ensures (fun h0 _ h1 -> red_c h0 a (U32.v i) /\ red_c h0 b (U32.v i) /\ live h1 a
+      /\ as_seq h1 a == fsum_spec (as_seq h0 a) (as_seq h0 b) (U32.v i)))
 let rec fsum_ a b i =
   if U32 (i =^ 0ul) then ()
   else (
     let i = U32 (i -^ 1ul) in
     let ai = a.(i) in let bi = b.(i) in
+    Math.Lemmas.pow2_double_sum n;
     a.(i) <- ai +^ bi;
     fsum_ a b i
   )
