crypto/bignum/Hacl.Bignum.Modulo.fsti
@@ -12,48 +12,68 @@ open Hacl.Bignum.Limb
 
 module U32 = FStar.UInt32
 
-(** Pure definition of the "add_zero" function **)
-val added_zero: mem -> felem -> mem -> felem -> Type0
+
+type seqelem = s:Seq.seq limb{Seq.length s = len}
+type seqelem_wide = s:Seq.seq wide{Seq.length s = len}
+
+val add_zero_pre: seqelem -> GTot Type0
+
+val add_zero_spec: s:seqelem{add_zero_pre s} -> Tot seqelem
 
 val add_zero:
   b:felem ->
   Stack unit
-    (requires (fun h -> live h b /\ reduced_after_mul h b))
-    (ensures (fun h0 _ h1 -> live h0 b /\ live h1 b /\ modifies_1 b h0 h1
-      /\ eval h1 b % prime = eval h0 b % prime
-      /\ added_zero h1 b h0 b
-      (* TODO: more fine grained condition or do an extra reduction step *)
-    ))
+    (requires (fun h -> live h b /\ add_zero_pre (as_seq h b)))
+    (ensures (fun h0 _ h1 -> live h0 b /\ add_zero_pre (as_seq h0 b) /\ live h1 b /\ modifies_1 b h0 h1
+      /\ as_seq h1 b == add_zero_spec (as_seq h0 b)
+      /\ eval h1 b % prime = eval h0 b % prime))
+
+val shift_reduce_pre: seqelem -> GTot Type0
 
 
-val reduced_after_sr: mem -> felem -> Type0
-val shift_reduced: mem -> felem -> mem -> felem -> Type0
+val shift_reduced_spec: s:seqelem{shift_reduce_pre s} -> Tot seqelem
 
 
 val shift_reduce:
   b:felem ->
   Stack unit
-    (requires (fun h -> live h b /\ reduced_after_mul h b))
-    (ensures (fun h0 _ h1 -> live h0 b /\ reduced_after_sr h1 b /\ modifies_1 b h0 h1 /\ live h1 b
-      /\ eval h1 b % prime = (eval h0 b * pow2 limb_size) % prime))
+    (requires (fun h -> live h b /\ shift_reduce_pre (as_seq h b)))
+    (ensures (fun h0 _ h1 -> live h0 b /\ shift_reduce_pre (as_seq h0 b) /\ modifies_1 b h0 h1 /\ live h1 b
+      /\ as_seq h1 b == shift_reduced_spec (as_seq h0 b)))
+
+
+val carry_top_pre: seqelem -> GTot Type0
+
+val carry_top_spec: s:seqelem{carry_top_pre s} -> Tot seqelem
 
 
 val carry_top:
   b:felem ->
   Stack unit
-  (requires (fun _ -> true))
-  (ensures (fun _ _ _ -> true))
+  (requires (fun h -> live h b /\ carry_top_pre (as_seq h b)))
+  (ensures (fun h0 _ h1 -> live h0 b /\ carry_top_pre (as_seq h0 b) /\ live h1 b /\ modifies_1 b h0 h1
+    /\ as_seq h1 b == carry_top_spec (as_seq h0 b)))
+
+
+val reduce_pre: seqelem -> GTot Type0
+
+val reduce_spec: s:seqelem{reduce_pre s} -> Tot seqelem
 
 
 val reduce:
   b:felem ->
   Stack unit
-  (requires (fun h -> true))
-  (ensures (fun _ _ _ -> true))
+  (requires (fun h -> live h b /\ reduce_pre (as_seq h b)))
+  (ensures (fun h0 _ h1 -> live h0 b /\ reduce_pre (as_seq h0 b) /\ live h1 b /\ modifies_1 b h0 h1
+    /\ as_seq h1 b == reduce_spec (as_seq h0 b)))
 
+val reduce_wide_pre: seqelem_wide -> GTot Type0
+
+val reduce_wide_spec: s:seqelem_wide{reduce_wide_pre s} -> Tot seqelem_wide
 
 val reduce_wide:
   b:felem_wide ->
   Stack unit
-    (requires (fun h -> true))
-    (ensures (fun _ _ _ -> true))
+    (requires (fun h -> live h b /\ reduce_wide_pre (as_seq h b)))
+    (ensures (fun h0 _ h1 -> live h0 b /\ reduce_wide_pre (as_seq h0 b) /\ live h1 b /\ modifies_1 b h0 h1
+      /\ as_seq h1 b == reduce_wide_spec (as_seq h0 b)))
