crypto/bignum/Hacl.Bignum.Predicates.fsti
@@ -17,20 +17,25 @@ let is_sum h1 (a:felem) h0 (b:felem) : GTot Type0 =
   /\ (forall (i:nat). {:pattern (v (get h1 a i))} i < len ==> v (get h1 a i) = v (get h0 a i) + v (get h0 b i))
 
 
-let 
-
 let is_difference h1 (a:felem) h0 (b:felem) : GTot Type0 =
   live h1 a /\ live h0 a /\ live h0 b
   /\ (forall (i:nat). {:pattern (v (get h1 a i))} i < len ==>
       v (get h1 a i) = v (get h0 b i) - v (get h0 b i))
 
 
-let is_sum_scalar_multiplication h1 a h0 b s 
+let is_sum_scalar_multiplication h1 (a:felem_wide) h0 (b:felem) s : GTot Type0 =
+  live h1 a /\ live h0 b
+  /\ (forall (i:nat). {:pattern (w (get h1 a i))} i < len ==> w (get h1 a i) = v (get h0 b i) * s)
+ 
 
-let is_multiplication hc c ha a hb b : GTot Type0 =
-  live hc c /\ live ha a /\ live hb b
-  /\ 
-let fsum_spec ha (a:felem) hb (b:felem)
+val is_shift_reduced: mem -> felem -> mem -> felem -> GTot Type0
+
+
+
+(* let is_multiplication hc c ha a hb b : GTot Type0 = *)
+(*   live hc c /\ live ha a /\ live hb b *)
+(*   /\  *)
+(* let fsum_spec ha (a:felem) hb (b:felem) *)
 
 
 (** Predicate associated to 'workable' bigintegers, restored after each bigint computation **)
@@ -42,3 +47,10 @@ val reduced_wide: h:mem -> b:felem_wide -> GTot Type0
 (** Predicate associated to 'workable' bigintegers, restored after each bigint computation **)
 val reducible: h:mem -> b:felem -> GTot Type0
 
+val lemma_sum_to_mul: h1:mem -> a:felem -> h0:mem -> b:felem -> Lemma
+  (requires (reduced_after_mul h0 a /\ reduced_after_mul h0 b /\ is_sum h1 a h0 b))
+  (ensures (reduced_before_mul_l h1 a))
+
+val lemma_difference_to_mul: h1:mem -> a:felem -> h0:mem -> b:felem -> Lemma
+  (requires (reduced_after_mul h0 a /\ reduced_after_mul h0 b /\ is_difference h1 a h0 b))
+  (ensures (reduced_before_mul_r h1 a))
